Checkpoint switching staged inv to use ae_inv_mut.

src/program_logic/staged_invariant.v
@@ -4,7 +4,7 @@ From stdpp Require Export namespaces.
 From iris.base_logic.lib Require Import wsat invariants saved_prop.
 From iris.algebra Require Import gmap.
 From iris.proofmode Require Import tactics.
-From Perennial.program_logic Require Export step_fupd_extra crash_token crash_weakestpre invariants_mutable ghost_var.
+From Perennial.program_logic Require Export step_fupd_extra crash_token crash_weakestpre ae_invariants_mutable ghost_var.
 Set Default Proof Using "Type".
 Import uPred.
 
@@ -24,8 +24,8 @@ Definition staged_done `{stagedG Σ} (γ: gname) : iProp Σ :=
   own γ (Cinr (to_agree ())).
 
 (* Schema:
-   Fixed: O => C, 1 => P, 2 => staged_done 1 γp;
-   Mutable: O => Qs, 1 => Qr; 2 => staged_done 1 γcancel; 3 => staged_pending γcancel *)
+   Fixed: O => C, 1 => P
+   Mutable: O => Qs, 1 => Qr *)
 
 Definition bi_sch_cfupd E E' P :=
   bi_sch_wand (bi_sch_var_fixed O) (bi_sch_fupd E E (bi_sch_fupd E' ∅ P)).
@@ -33,116 +33,18 @@ Definition bi_sch_cfupd E E' P :=
 Definition bi_sch_staged_fupd (E: coPset) :=
   bi_sch_persistently
     (bi_sch_wand (bi_sch_var_mut O)
-                 (bi_sch_cfupd E ∅ (bi_sch_sep (bi_sch_or (bi_sch_var_fixed 1) (bi_sch_var_fixed 2))
-                                               (bi_sch_var_mut 1)))).
-
-Definition bi_sch_True := bi_sch_pure True.
-Definition bi_sch_inv' (N: namespace) (P: bi_schema) : bi_schema :=
-  bi_sch_persistently
-    (bi_sch_forall coPset
-       (λ E : coPset,
-              bi_sch_wand (bi_sch_pure (↑N ⊆ E))
-                          (bi_sch_fupd E (E ∖ ↑N)
-                                       (bi_sch_sep P
-                                                   (bi_sch_wand P
-                                                                (bi_sch_fupd (E ∖ ↑N) E bi_sch_True)))))).
-Definition bi_sch_inv (N: namespace) (P: bi_schema) : bi_schema :=
-  bi_sch_inv' N (bi_sch_later P).
-
-(* Four states for the inner invariant? *)
-
-(* active, full => Qs
-   cancelled => ?
-   crashed => C * (...)
-
-Definition inner_inv Qs Qr γcancel γp γqr :=
-  (Qs ∨ (C * (Qr ∨ staged_done γqr) * (P ∨ staged_done γp))) ∨ staged_done γcancel *)
-
-
-Definition bi_sch_staged_cases_noncancel :=
-  bi_sch_or (bi_sch_var_mut O)
-            (bi_sch_sep (bi_sch_var_mut 1) (bi_sch_sep (bi_sch_var_fixed O)
-                                                       (bi_sch_or (bi_sch_var_fixed 1) (bi_sch_var_fixed 2)))).
+                 (bi_sch_cfupd E ∅ (bi_sch_sep (bi_sch_var_fixed 1) (bi_sch_var_mut 1)))).
 
 Definition bi_sch_staged_cases :=
-  bi_sch_or (bi_sch_staged_cases_noncancel)
-            (bi_sch_var_mut 2).
+  bi_sch_or (bi_sch_var_mut O)
+            (bi_sch_sep (bi_sch_var_mut 1) (bi_sch_sep (bi_sch_var_fixed O) (bi_sch_var_fixed 1))).
 
-Definition bi_sch_staged_cases_inv_wrapped N :=
-  bi_sch_inv' N bi_sch_staged_cases.
+Definition bi_sch_staged E :=
+  bi_sch_sep (bi_sch_staged_fupd E) (bi_sch_staged_cases).
 
-Definition bi_sch_pending_done :=
-  bi_sch_persistently (bi_sch_wand (bi_sch_var_mut 2)
-                                   (bi_sch_wand (bi_sch_var_mut 3) (bi_sch_fupd ∅ ∅ (bi_sch_pure False)))).
-
-Definition bi_sch_staged N E :=
-  bi_sch_sep (bi_sch_staged_fupd E)
-             (bi_sch_sep (bi_sch_pending_done)
-                         (bi_sch_sep (bi_sch_var_mut 3)
-                                     (bi_sch_staged_cases_inv_wrapped N))).
-
-Definition inv_lvl `{!invG Σ} (k: nat) (N : namespace) (P : iProp Σ) : iProp Σ :=
-  □ ∀ E, ⌜↑N ⊆ E⌝ -∗ |k={E,E ∖ ↑N}=> ▷ P ∗ (▷ P -∗ |k={E ∖ ↑N,E}=> True).
-
-Lemma bi_sch_inv_interp `{!invG Σ} k N Ps Qs sch P:
-  bi_schema_interp (S k) Ps Qs sch ≡ (▷ P)%I →
-  bi_schema_interp (S k) Ps Qs (bi_sch_inv' N sch) ≡ inv_lvl k N P.
-Proof.
-  intros Hinterp. rewrite /inv_lvl.
-  remember (S k) as k' eqn:Hlvl.
-  repeat (rewrite ?Hinterp; rewrite ?bi_schema_interp_unfold //=).
-  rewrite intuitionistically_into_persistently.
-  do 2 f_equiv. intros E.
-  repeat (rewrite bi_schema_interp_unfold //=; rewrite ?Hinterp).
-  rewrite ?uPred_fupd_level_eq /uPred_fupd_level_def /bi_except_0 Hlvl.
-  auto.
-Qed.
-
-Lemma bi_sch_staged_interp `{!invG Σ, !crashG Σ, !stagedG Σ} N E k γp γcancel Qs Qr P :
-  bi_schema_interp (S k)
-                   (bi_later <$> [C; P; staged_done γp])
-                   (bi_later <$> [Qs; Qr; staged_done γcancel; staged_pending (1/2)%Qp γcancel])
-                   (bi_sch_staged N E)
-  ⊣⊢ □ (▷ Qs -∗ ▷ C -∗ |k={E}=> |k={∅, ∅}=> (▷ P ∨ ▷ staged_done γp) ∗ ▷ Qr) ∗
-     □ (▷ staged_done γcancel -∗ ▷ staged_pending (1/2)%Qp γcancel -∗ |k={∅}=> False) ∗
-     ▷ staged_pending (1/2)%Qp γcancel ∗
-     inv_lvl k N ((Qs ∨ (Qr ∗ C ∗ (P ∨ staged_done γp))) ∨ staged_done γcancel)%I.
-Proof.
-  remember (S k) as k' eqn:Hlvl.
-  do 2 rewrite bi_schema_interp_unfold //=.
-  do 2 rewrite bi_schema_interp_unfold //=.
-  do 2 rewrite bi_schema_interp_unfold //=.
-  rewrite Hlvl.
-  erewrite bi_sch_fupd_interp; last first.
-  { eapply bi_sch_fupd_interp. eauto. }
-  do 1 rewrite bi_schema_interp_unfold.
-  do 1 rewrite bi_schema_interp_unfold.
-  do 1 rewrite bi_schema_interp_unfold.
-  do 1 rewrite bi_schema_interp_unfold.
-  do 1 rewrite bi_schema_interp_unfold.
-  do 1 rewrite bi_schema_interp_unfold.
-  do 1 rewrite (bi_schema_interp_unfold _ _ _ (bi_sch_sep _ _)).
-  rewrite (bi_sch_inv_interp); last first.
-  { repeat (rewrite ?bi_schema_interp_unfold /=).
-    rewrite -?later_sep -?later_or /=.
-    rewrite -?later_sep -?later_or /=.
-    reflexivity. }
-  f_equiv; [| f_equiv].
-  - repeat (rewrite ?bi_schema_interp_unfold intuitionistically_into_persistently //=).
-  - rewrite /bi_sch_pending_done.
-    do 1 rewrite bi_schema_interp_unfold.
-    do 1 rewrite bi_schema_interp_unfold.
-    do 1 rewrite bi_schema_interp_unfold.
-    do 1 rewrite bi_schema_interp_unfold.
-    erewrite bi_sch_fupd_interp; last first.
-    { rewrite //=. }
-    do 1 rewrite bi_schema_interp_unfold //= ?intuitionistically_into_persistently. auto.
-Qed.
-
-(*
-Lemma bi_sch_staged_interp `{!invG Σ, !crashG Σ, !stagedG Σ} E k γ Qs Qr P :
-  bi_schema_interp (S k) (bi_later <$> [C; P; staged_done γ]) (bi_later <$> [Qs; Qr]) (bi_sch_staged E)
-  ⊣⊢ (□ (▷ Qs -∗ ▷ C -∗ |k={E}=> |k={∅, ∅}=> ▷ P ∗ ▷ Qr) ∗ (▷ Qs ∨ (▷ Qr ∗ ▷ C ∗ ▷ staged_done γ)))%I.
+Lemma bi_sch_staged_interp `{!invG Σ, !crashG Σ, !stagedG Σ} E k Qs Qr P :
+  bi_schema_interp (S k) (bi_later <$> [C; P]) (bi_later <$> [Qs; Qr]) (bi_sch_staged E)
+  ⊣⊢ (□ (▷ Qs -∗ ▷ C -∗ |k={E}=> |k={∅, ∅}=> ▷ P ∗ ▷ Qr) ∗ (▷ Qs ∨ (▷ Qr ∗ ▷ C ∗ ▷ P)))%I.
 Proof.
   remember (S k) as k' eqn:Hlvl.
   repeat (rewrite ?bi_schema_interp_unfold //=).
@@ -150,121 +52,13 @@ Proof.
   rewrite Hlvl /bi_except_0 intuitionistically_into_persistently.
   done.
 Qed.
-*)
 
-Lemma bi_sch_staged_interp_weak `{!invG Σ, !crashG Σ, !stagedG Σ} N E k γ Qs_mut P :
-  bi_schema_interp (S k) (bi_later <$> [C; P; staged_done γ]) (bi_later <$> Qs_mut) (bi_sch_staged N E)
-  ⊣⊢ let Qs := default emp%I (Qs_mut !! O) in
-     let Qr := default emp%I (Qs_mut !! 1) in
-     let cancel_done := default emp%I (Qs_mut !! 2) in
-     let cancel_pending := default emp%I (Qs_mut !! 3) in
-     □ (▷ Qs -∗ ▷ C -∗ |k={E}=> |k={∅, ∅}=> (▷ P ∨ ▷ staged_done γ) ∗ ▷ Qr) ∗
-     □ (▷ cancel_done -∗ ▷cancel_pending -∗ |k={∅}=> False) ∗
-     ▷ cancel_pending ∗
-     inv_lvl k N ((Qs ∨ (Qr ∗ C ∗ (P ∨ staged_done γ))) ∨ cancel_done)%I.
-Proof.
-  remember (S k) as k' eqn:Hlvl.
-  do 2 rewrite bi_schema_interp_unfold //=.
-  do 2 rewrite bi_schema_interp_unfold //=.
-  do 2 rewrite bi_schema_interp_unfold //=.
-  rewrite Hlvl.
-  erewrite bi_sch_fupd_interp; last first.
-  { eapply bi_sch_fupd_interp. eauto. }
-  do 1 rewrite bi_schema_interp_unfold.
-  do 1 rewrite bi_schema_interp_unfold.
-  do 1 rewrite bi_schema_interp_unfold.
-  do 1 rewrite bi_schema_interp_unfold.
-  do 1 rewrite bi_schema_interp_unfold.
-  do 1 rewrite bi_schema_interp_unfold.
-  do 1 rewrite (bi_schema_interp_unfold _ _ _ (bi_sch_sep _ _)).
-  f_equiv; [| f_equiv; [| f_equiv]].
-  - repeat (rewrite ?bi_schema_interp_unfold intuitionistically_into_persistently //=).
-    rewrite ?list_lookup_fmap.
-    destruct (Qs_mut !! O); destruct (Qs_mut !! 1); destruct (Qs_mut !! 2) => //=;
-    rewrite ?later_emp; auto.
-  - rewrite /bi_sch_pending_done.
-    do 1 rewrite bi_schema_interp_unfold.
-    do 1 rewrite bi_schema_interp_unfold.
-    do 1 rewrite bi_schema_interp_unfold.
-    do 1 rewrite bi_schema_interp_unfold.
-    erewrite bi_sch_fupd_interp; last first.
-    { rewrite //=. }
-    do 1 rewrite bi_schema_interp_unfold //= ?intuitionistically_into_persistently. auto.
-    rewrite ?list_lookup_fmap.
-    destruct (Qs_mut !! 2); destruct (Qs_mut !! 3) => //=;
-    rewrite ?later_emp; auto.
-  - do 1 rewrite bi_schema_interp_unfold //= ?intuitionistically_into_persistently. auto.
-    rewrite ?list_lookup_fmap.
-    destruct (Qs_mut !! 3);
-    rewrite ?later_emp; auto.
-  - eapply bi_sch_inv_interp => //=.
-    rewrite ?list_lookup_fmap.
-    destruct (Qs_mut !! O); [| rewrite -{1}later_emp];
-    (destruct (Qs_mut !! 1); [| rewrite -{2}later_emp];
-     (destruct (Qs_mut !! 2); [| rewrite -{3}later_emp])) => //=;
-    repeat (rewrite -?later_sep -?later_or /=) => //=.
-Qed.
-
-(*
-Lemma bi_sch_staged_interp_weak `{!invG Σ, !crashG Σ, !stagedG Σ} N E k γ Qs_mut P :
-  bi_schema_interp (S k) (bi_later <$> [C; P; staged_done γ]) (bi_later <$> Qs_mut) (bi_sch_staged N E)
+Lemma bi_sch_staged_interp_weak `{!invG Σ, !crashG Σ, !stagedG Σ} E k Qs_mut P :
+  bi_schema_interp (S k) (bi_later <$> [C; P]) (bi_later <$> Qs_mut) (bi_sch_staged E)
   ⊣⊢ let Qs := default emp%I (bi_later <$> (Qs_mut !! O)) in
      let Qr := default emp%I (bi_later <$> (Qs_mut !! 1)) in
-     let cancel_done := default emp%I (bi_later <$> (Qs_mut !! 2)) in
-     let cancel_pending := default emp%I (bi_later <$> (Qs_mut !! 3)) in
-     □ (Qs -∗ ▷ C -∗ |k={E}=> |k={∅, ∅}=> ▷ P ∗ Qr) ∗
-     □ (cancel_done -∗ cancel_pending -∗ |k={∅}=> False) ∗
-     cancel_pending ∗
-     inv_lvl k N ((Qs ∨ (Qr ∗ C ∗ (P ∨ staged_done γ))) ∨ cancel_done)%I.
+     (□ (Qs -∗ ▷ C -∗ |k={E}=> |k={∅, ∅}=> ▷ P ∗ Qr) ∗ (Qs ∨ (Qr ∗ ▷ C ∗ ▷ P)))%I.
 Proof.
-  remember (S k) as k' eqn:Hlvl.
-  do 2 rewrite bi_schema_interp_unfold //=.
-  do 2 rewrite bi_schema_interp_unfold //=.
-  do 2 rewrite bi_schema_interp_unfold //=.
-  rewrite Hlvl.
-  erewrite bi_sch_fupd_interp; last first.
-  { eapply bi_sch_fupd_interp. eauto. }
-  do 1 rewrite bi_schema_interp_unfold.
-  do 1 rewrite bi_schema_interp_unfold.
-  do 1 rewrite bi_schema_interp_unfold.
-  do 1 rewrite bi_schema_interp_unfold.
-  do 1 rewrite (bi_schema_interp_unfold _ _ _ (bi_sch_sep _ _)).
-  f_equiv; [| f_equiv; [| f_equiv]].
-  - repeat (rewrite ?bi_schema_interp_unfold intuitionistically_into_persistently //=).
-    rewrite ?list_lookup_fmap.
-    destruct (Qs_mut !! O); destruct (Qs_mut !! 1); destruct (Qs_mut !! 2); auto.
-  - rewrite /bi_sch_pending_done.
-    do 1 rewrite bi_schema_interp_unfold.
-    do 1 rewrite bi_schema_interp_unfold.
-    do 1 rewrite bi_schema_interp_unfold.
-    do 1 rewrite bi_schema_interp_unfold.
-    erewrite bi_sch_fupd_interp; last first.
-    { rewrite //=. }
-    do 1 rewrite bi_schema_interp_unfold //= ?intuitionistically_into_persistently. auto.
-    rewrite ?list_lookup_fmap.
-    destruct (Qs_mut !! O); destruct (Qs_mut !! 1); destruct (Qs_mut !! 2); auto.
-  - do 1 rewrite bi_schema_interp_unfold //= ?intuitionistically_into_persistently. auto.
-    rewrite ?list_lookup_fmap.
-    destruct (Qs_mut !! O); destruct (Qs_mut !! 1); destruct (Qs_mut !! 2); auto.
-  - eapply bi_sch_inv_interp => //=.
-    rewrite ?list_lookup_fmap.
-    destruct (Qs_mut !! O); destruct (Qs_mut !! 1); destruct (Qs_mut !! 2); auto => //=.
-    repeat (rewrite //= -?later_emp -?later_sep -?later_or /=).
-    repeat (rewrite //= -?later_emp -?later_sep -?later_or /=).
-    rewrite -?later_sep -?later_or /=. reflexivity. auto.
-    rewrite -?later_sep -?later_or /=.
-    reflexivity. }
-  f_equiv; [| f_equiv].
-  - repeat (rewrite ?bi_schema_interp_unfold intuitionistically_into_persistently //=).
-  - rewrite /bi_sch_pending_done.
-    do 1 rewrite bi_schema_interp_unfold.
-    do 1 rewrite bi_schema_interp_unfold.
-    do 1 rewrite bi_schema_interp_unfold.
-    do 1 rewrite bi_schema_interp_unfold.
-    erewrite bi_sch_fupd_interp; last first.
-    { rewrite //=. }
-    do 1 rewrite bi_schema_interp_unfold //= ?intuitionistically_into_persistently. auto.
-Qed.
   remember (S k) as k' eqn:Hlvl.
   repeat (rewrite ?bi_schema_interp_unfold //=).
   rewrite /cfupd ?uPred_fupd_level_eq /uPred_fupd_level_def.
@@ -272,29 +66,17 @@ Qed.
   rewrite /default. rewrite ?list_lookup_fmap.
   destruct (Qs_mut !! O); destruct (Qs_mut !! 1); auto.
 Qed.
-*)
 
 Section staged_inv_defns.
 
   Context `{!invG Σ, !crashG Σ, !stagedG Σ}.
 
-Definition staged_inv (k: nat) (N1 N2: namespace) E (γ: gname) (P: iProp Σ) : iProp Σ :=
-  inv_mut k N1 (bi_sch_staged N2 E) [C; P; staged_done γ].
+Definition staged_inv (k: nat) E (γ: gname) (P: iProp Σ) : iProp Σ :=
+  ae_inv_mut k (bi_sch_staged E) [C; (P ∨ staged_done γ)%I].
 
-Definition staged_value (k: nat) (N1 N2: namespace) E (γp: gname) (Qs Qr P: iProp Σ) :=
-  (∃ γcancel γr,
-  staged_pending 1%Qp γr ∗
-  staged_pending (1/2)%Qp γcancel ∗
-  inv N2 ((Qs ∨ ((Qr ∨ staged_done γr) ∗ C ∗ (P ∨ staged_done γp))) ∨ staged_done γcancel) ∗
-  inv_mut_full k N1 (bi_sch_staged N2 E) [Qs; (Qr ∨ (staged_done γr)); staged_done γcancel;
-                                                 staged_pending (1/2)%Qp γcancel]
-                                         [C; P; staged_done γp])%I.
-
-Definition staged_value_disc (N2: namespace) (γp: gname) (Qs Qr P: iProp Σ) :=
-  (∃ γcancel γr,
-  staged_pending 1%Qp γr ∗
-  staged_pending (1/2)%Qp γcancel ∗
-  inv N2 ((Qs ∨ ((Qr ∨ staged_done γr) ∗ C ∗ (P ∨ staged_done γp))) ∨ staged_done γcancel))%I.
+Definition staged_value (k: nat) E (γp: gname) (b: bool) (Qs Qr P: iProp Σ) :=
+  (∃ γr, (if b then staged_pending 1%Qp γr else staged_done γr) ∗
+  ae_inv_mut_full k (bi_sch_staged E) [Qs; (Qr ∨ staged_done γr)] [C; (P ∨ staged_done γp)%I])%I.
 
 End staged_inv_defns.
 
@@ -303,14 +85,6 @@ Context `{!invG Σ, !stagedG Σ, !crashG Σ}.
 Implicit Types i : positive.
 Implicit Types N : namespace.
 Implicit Types P Q R : iProp Σ.
-
-Lemma staged_value_into_disc k N1 N2 E γp Qs Qr P :
-  staged_value k N1 N2 E γp Qs Qr P -∗
-  <disc> staged_value_disc N2 γp Qs Qr P.
-Proof.
-  iDestruct 1 as (??) "(Hp1&Hp2&#Hinv&_)".
-  iModIntro. iExists _, _. by iFrame.
-Qed.
 
 (*
 Global Instance staged_contractive k N E E' γ : Contractive (staged_inv k N E E' γ).
@@ -329,7 +103,7 @@ Global Instance staged_proper N E E' γ γ' : Proper ((⊣⊢) ==> (⊣⊢)) (st
 Proof. apply ne_proper, _. Qed.
 *)
 
-Global Instance staged_persistent k N E γ P : Persistent (staged_inv k N1 N2 E γ P).
+Global Instance staged_persistent k E γ P : Persistent (staged_inv k E γ P).
 Proof. rewrite /staged_inv. apply _. Qed.
 
 Lemma pending_done q γ: staged_pending q γ -∗ staged_done γ -∗ False.
@@ -347,24 +121,6 @@ Proof.
   done.
 Qed.
 
-(*
-Lemma staged_inv_iff N E E' γ γ' P Q :
-  ▷ □ (P ↔ Q) -∗
-  staged_inv N E E' γ γ' P -∗
-  staged_inv N E E' γ γ' Q.
-Proof.
-  iIntros "#HPQ". iApply inv_iff. iNext. iAlways. iSplit.
-  - iIntros "H". iDestruct "H" as (?? P0 P0') "(?&?&?&#HP0&Hcase)". iExists _, _, P0, P0'. iFrame.
-    iAlways. iIntros. iSpecialize ("HP0" with "[$] [$]").
-    iApply (step_fupdN_inner_wand' with "HP0"); eauto.
-    iIntros "(?&$)". by iApply "HPQ".
-  - iIntros "H". iDestruct "H" as (?? P0 P0') "(?&?&?&#HP0&Hcase)". iExists _, _, P0, P0'. iFrame.
-    iAlways. iIntros. iSpecialize ("HP0" with "[$] [$]").
-    iApply (step_fupdN_inner_wand' with "HP0"); eauto.
-    iIntros "(?&$)". by iApply "HPQ".
-Qed.
-*)
-
 Lemma pending_alloc:
   ⊢ |==> ∃ γ, staged_pending 1 γ.
 Proof.
@@ -380,183 +136,119 @@ Lemma pending_join γ:
  staged_pending (1/2)%Qp γ ∗ staged_pending (1/2)%Qp γ ⊢  staged_pending 1 γ.
 Proof. by rewrite /staged_pending -own_op -Cinl_op frac_op' Qp_div_2. Qed.
 
-Lemma staged_inv_alloc k N1 N2 E E' P Q Qr:
+Lemma staged_inv_alloc k E E' P Q Qr:
   ▷ Q ∗ □ (C -∗ ▷ Q -∗ ▷ P ∗ ▷ Qr) -∗ |(S k)={E}=>
-  ∃ γ, staged_inv (S k) N1 N2 E' γ P ∗ staged_value (S k) N1 N2 E' γ Q Qr P ∗ staged_pending 1%Qp γ.
+  ∃ γ, staged_inv (S k) E' γ P ∗ staged_value (S k) E' γ true Q Qr P ∗ staged_pending 1%Qp γ.
 Proof.
-  iMod (pending_alloc) as (γp) "Hp".
-  iMod (pending_alloc) as (γcancel) "Hc".
+  iMod (pending_alloc) as (γ) "H".
   iMod (pending_alloc) as (γr) "Hr".
   iIntros "(HQ&#HQP)".
-  iMod (inv_alloc' _ N2 E
-        (((Q ∨ ((Qr ∨ staged_done γr) ∗ C ∗ (P ∨ staged_done γp))) ∨ staged_done γcancel))%I
-        with "[HQ]") as "#Hinv0".
-  { repeat iLeft. auto. }
-
-  iDestruct (pending_split with "Hc") as "(Hc1&Hc2)".
-  iMod (inv_mut_alloc (S k) N1 E (bi_sch_staged N2 E')
-                   [C; P; staged_done γp]
-                   [Q; (Qr ∨ staged_done γr)%I; staged_done γcancel; staged_pending (1/2)%Qp γcancel]
-          with "[Hc1]")
+  iMod (ae_inv_mut_alloc (S k) E (bi_sch_staged E')
+                   [C; (P ∨ staged_done γ)%I]
+                   [Q; (Qr ∨ staged_done γr)%I]
+          with "[HQ]")
       as "(#Hi&Hmut)".
   { simpl fmap. rewrite bi_sch_staged_interp.
-    iSplitL ""; [| iSplitL ""].
+    iSplitL "".
     - iModIntro. iIntros "HQ >HC". iModIntro.
       iApply fupd_level_mask_weaken; first by set_solver+.
       iDestruct ("HQP" with "[$] [$]") as "($&$)".
-    - iModIntro. iIntros ">H1 >H2". iModIntro. iApply (pending_done with "[$] [$]").
-    - iFrame.
-      rewrite /inv_lvl.
-      iModIntro. iIntros (E0 Hsub).
-      iInv "Hinv0" as "H" "Hclo".
-      iModIntro. iFrame.
+    - iLeft. eauto.
   }
-  iModIntro. iExists _. iFrame "# ∗". iExists _, _. iFrame "# ∗".
+  iModIntro. iExists _. iFrame "# ∗". iExists _; eauto. iFrame.
 Qed.
 
-Lemma staged_inv_open_modify E k N1 N2 E1 γ P Q Qr:
-  N1 ## N2 →
-  ↑N1 ⊆ E →
-  ↑N2 ⊆ E →
-  staged_value (S k) N1 N2 E1 γ Q Qr P -∗ |(S k)={E,E∖↑N1}=>
-  (▷ Q ∗ (∀ Q' Qr', ▷ Q' ∗
-   □ (▷ Q' -∗ |C={E1, ∅}_k=> P ∗ Qr') -∗ |(S k)={E∖↑N1,E}=> staged_value (S k) N1 N2 E1 γ Q' Qr' P)) ∨
-  (▷ Qr ∗ C ∗ |(S k)={E∖↑N1, E}=> staged_value (S k) N1 N2 E1 γ Q True P).
+Lemma staged_inv_open_modify_ae E k E1 γ P Q Qr Q' Qr' R:
+  staged_value (S k) E1 γ true Q Qr P -∗
+  □ (▷ Q' -∗ |C={E1, ∅}_k=> P ∗ Qr') -∗
+  (▷ Q -∗ |k={E}=> ▷ Q' ∗ R) -∗
+  |(S k)={E}=> (R ∗ staged_value (S k) E1 γ true Q' Qr' P) ∨
+               (▷ Qr ∗ C ∗ staged_value (S k) E1 γ false Q' Qr' P).
 Proof.
-  (* XXX: clean this up, the encoding is very silly in some ways *)
-  iIntros (???) "Hval".
-  iDestruct "Hval" as (??) "(Hqr&Hcancel&#Hinv&Hval)".
-  iMod (inv_mut_full_acc with "Hval") as "(Hinterp&Hclo)"; auto.
-  iInv "Hinv" as "H" "Hclo'".
-  iDestruct "H" as "[HQ|>Hfalse]"; last first.
-  { iDestruct (pending_done with "[$] [$]") as %[]. }
-  iDestruct (bi_sch_staged_interp with "Hinterp") as "(#Hwand&_&>Hcancel2&_)".
+  iIntros "Hval #Hwand Hshift".
+  rewrite /staged_value/=.
+  iDestruct "Hval" as (γr) "(Hγr&Hval)" => //=.
+  iMod (ae_inv_mut_full_acc _ _ _ _ ([Q'; (Qr' ∨ staged_done γr)%I]) _
+                            ((R ∗ staged_pending 1%Qp γr)  ∨ (▷ Qr ∗ C ∗ staged_done γr))%I
+          with "Hval [Hγr Hshift]") as "(HR&Hclo)";
+    last first.
+  { iModIntro. iDestruct "Hclo" as "[(Hr&?)|(?&?&?)]".
+    - iLeft. iFrame. iExists _. iFrame; eauto.
+    - iRight. iFrame. iExists _. iFrame; eauto.
+  }
+  iIntros "HQ".
+  iDestruct (bi_sch_staged_interp with "HQ") as "(#Hwand'&HQ)".
   iDestruct "HQ" as "[HQ|HQ]".
-  - iDestruct (pending_join with "[$Hcancel $Hcancel2]") as "Hcancel".
-    iMod (pending_upd_done with "Hcancel") as "Hcancel".
-    iMod ("Hclo'" with "[Hcancel]") as "_".
-    { iRight. eauto. }
-    iModIntro. iLeft. iFrame. iIntros (Q' Qr') "(HQ'&#Hwand')".
-    iClear "Hinv".
-    iMod (pending_alloc) as (γcancel') "Hc".
-    iMod (inv_alloc' _ N2 _
-        (((Q' ∨ ((Qr' ∨ staged_done γr) ∗ C ∗ (P ∨ staged_done γ))) ∨ staged_done γcancel'))%I
-        with "[HQ']") as "#Hinv0".
-    { repeat iLeft. auto. }
-    iDestruct (pending_split with "Hc") as "(Hc1&Hc2)".
-    iMod ("Hclo" $! [Q'; (Qr' ∨ staged_done γr)%I;
-                     staged_done γcancel'; staged_pending (1/2)%Qp γcancel'] with "[Hc1]").
-    { rewrite bi_sch_staged_interp.
-      iSplitL ""; [| iSplitL ""].
-      - iIntros "!> HQ' >HC".  iMod ("Hwand'" with "[$] [$]") as "H".
-        iModIntro. iMod "H" as "($&$)". auto.
-      - iModIntro. iIntros ">H1 >H2". iModIntro. iApply (pending_done with "[$] [$]").
-      - iFrame.
-        rewrite /inv_lvl.
-        iModIntro. iIntros (E0 Hsub).
-        iInv "Hinv0" as "H" "Hclo".
-        iModIntro. iFrame.
+  - iMod ("Hshift" with "HQ") as "(HQ&HR)".
+    iSplitL "HQ".
+    { iModIntro. erewrite bi_sch_staged_interp.
+      iSplitL "".
+      { iIntros "!> HQ' >HC". iMod ("Hwand" with "[$] [$]") as "H".
+        iModIntro. by iMod "H" as "($&$)".
+      }
+      by iLeft.
     }
-    iModIntro. iExists _, _. iFrame "# ∗".
-  - iRight. iDestruct "HQ" as "(HQr&>#HC&HP)".
-    iFrame "HC".
-    iDestruct "HQr" as "[HQr|>Hfalse]"; last first.
-    { iDestruct (pending_done with "Hqr [$]") as %[]. }
-    iMod (pending_upd_done with "Hqr") as "Hqr".
-    iDestruct (pending_join with "[$Hcancel $Hcancel2]") as "Hcancel".
-    iMod (pending_upd_done with "Hcancel") as "Hcancel".
-    iMod ("Hclo'" with "[Hcancel]") as "_".
-    { iRight. eauto. }
-    iModIntro. iFrame.
-    iClear "Hinv".
-    iMod (pending_alloc) as (γr') "Hqr'".
-    iMod (pending_alloc) as (γcancel') "Hc".
-    iMod (inv_alloc' _ N2 _
-        (((Q ∨ ((True ∨ staged_done γr') ∗ C ∗ (P ∨ staged_done γ))) ∨ staged_done γcancel'))%I
-        with "[HP]") as "#Hinv0".
-    { iLeft. iRight. iFrame "# ∗". by iLeft. }
-    iDestruct (pending_split with "Hc") as "(Hc1&Hc2)".
-    iMod ("Hclo" $! [Q; (True ∨ staged_done γr')%I;
-                     staged_done γcancel'; staged_pending (1/2)%Qp γcancel'] with "[Hc2]").
+    iModIntro. iLeft. iFrame.
+  - iDestruct "HQ" as "(HQr&>#HC&HP)".
+    iDestruct "HQr" as "[HQR|>Hfalse]"; last first.
+    { iDestruct (pending_done with "[$] [$]") as %[]. }
+    iMod (pending_upd_done with "Hγr") as "#Hγr".
+    iModIntro.
+    iSplitL "Hshift HP".
     { rewrite bi_sch_staged_interp.
-      iSplitL ""; [| iSplitL ""].
-      - iIntros "!> HQ' _". iMod ("Hwand" with "[$] [$]") as "H".
-        iModIntro. iMod "H" as "($&?)". iModIntro. by iLeft.
-      - iModIntro. iIntros ">H1 >H2". iModIntro. iApply (pending_done with "[$] [$]").
-      - iFrame.
-        rewrite /inv_lvl.
-        iModIntro. iIntros (E0 Hsub).
-        iInv "Hinv0" as "H" "Hclo".
-        iModIntro. iFrame.
+      iSplitL "".
+      { iIntros "!> HQ' _". iMod ("Hwand" with "[$] [$]") as "H". iModIntro.
+        by iMod "H" as "($&$)". }
+      iRight. iFrame. eauto.
     }
-    iModIntro.  iExists _, _. iFrame "# ∗".
+    iRight. iFrame "# ∗".
 Qed.
 
-Lemma staged_inv_disc_open_crash k E N2 γ P Q Qr:
-  ↑N2 ⊆ E →
-  □ (▷ Q -∗ ▷ C -∗ |k={E∖↑N2}=> |k={∅, ∅}=> ▷ P ∗ ▷ Qr) -∗
-  staged_value_disc N2 γ Q Qr P -∗ C -∗ |k={E,E}=> ▷ Qr.
+Lemma staged_inv_open_crash k E γ P Q Qr:
+  □ (▷ Q -∗ ▷ C -∗ |k={E}=> |k={∅, ∅}=> ▷ P ∗ ▷ Qr) -∗
+  staged_value (S k) E γ true Q Qr P -∗ C -∗ |(S k)={E,E}=> ▷ Qr.
 Proof.
-  iIntros (?) "#Hwand".
-  iDestruct 1 as (??) "(Hqr&Hqc&#Hinv)".
-  iInv "Hinv" as "H" "Hclo'".
-  iDestruct "H" as "[HQ|>Hfalse]"; last first.
-  { iDestruct (pending_done with "[$] [$]") as %[]. }
-  iIntros "#HC".
-  iDestruct "HQ" as "[HQ|HQr]".
+  iIntros "#Hwand".
+  iDestruct 1 as (?) "(Hγr&Hval)". iIntros "#HC".
+  iMod (ae_inv_mut_full_acc _ _ _ _ ([Q; (Qr ∨ staged_done γr)%I]) _
+                            (▷ Qr)%I
+          with "Hval [Hγr]") as "(HR&Hclo)";
+    last first.
+  { iModIntro. auto. }
+  iIntros "HQ".
+  iDestruct (bi_sch_staged_interp with "HQ") as "(#Hwand'&HQ)".
+  iDestruct "HQ" as "[HQ|HQ]".
   - iMod ("Hwand" with "[$] [$]") as "H".
     iMod (fupd_level_intro_mask' _ ∅) as "Hclo''"; first by set_solver+.
     iMod ("H") as "(HP&$)".
     iMod "Hclo''" as "_".
-    iMod (pending_upd_done with "Hqr") as "Hqr".
-    iMod ("Hclo'" with "[HP Hqr]").
-    { iNext. iLeft. iRight. by iFrame. }
+    iMod (pending_upd_done with "Hγr") as "Hγr".
+    iModIntro. rewrite bi_sch_staged_interp. iFrame "#". iRight. iFrame.
+  - iDestruct "HQ" as "([HQr|>Hfalse]&_&HP)"; last first.
+    { iDestruct (pending_done with "Hγr [$]") as %[]. }
+    iMod (pending_upd_done with "Hγr") as "#Hγr".
+    iModIntro.
+    iSplitL "HP".
+    { rewrite bi_sch_staged_interp.
+      iSplitL "".
+      { iIntros "!> HQ' _". iMod ("Hwand" with "[$] [$]") as "H". iModIntro.
+        by iMod "H" as "($&$)". }
+      iRight. iFrame. eauto.
+    }
     eauto.
-  - iDestruct "HQr" as "([HQr|>Hfalse]&_&HP)"; last first.
-    { iDestruct (pending_done with "Hqr [$]") as %[]. }
-    iMod (pending_upd_done with "Hqr") as "Hqr".
-    iMod ("Hclo'" with "[HP Hqr]").
-    { iNext. iLeft. iRight. by iFrame. }
-    by iFrame.
 Qed.
 
-(*
-Lemma staged_inv_NC_open E k N E1 E2 γ P Q Qr:
-  ↑N1 ⊆ E →
-  E2 ⊆ E1 →
-  NC ∗
-  staged_value (S k) N1 N2 E1 γ Q Qr P -∗ |(S k)={E,E∖↑N}=>
-  (▷ Q ∗ (∀ Q' Qr', ▷ Q' ∗
-   □ (▷ Q' -∗ |C={E1, ∅}_k=> ▷ P ∗ ▷ Qr') -∗ |(S k)={E∖↑N,E}=> staged_value (S k) N E1 γ Q' Qr' P)).
-Proof.
-  iIntros (??) "(HNC&Hval)".
-  iMod (staged_inv_open with "[$]") as "[H|(_&HC&_)]"; auto.
-  iDestruct (NC_C with "[$] [$]") as %[].
-Qed.
-*)
-
-Lemma staged_inv_weak_open E k N1 N2 E1 γ P:
-  E1 ⊆ E ∖ ↑N1 ∖ ↑N2 →
-  N1 ## N2 →
-  ↑N1 ⊆ E →
-  ↑N2 ⊆ E →
-  staged_inv (S k) N1 N2 E1 γ P ∗
+Lemma staged_inv_weak_open E k E1 γ P:
+  E1 ⊆ E →
+  staged_inv (S k) E1 γ P ∗
   staged_pending 1%Qp γ ∗
   C -∗ |(S k)={E,E}=> ▷ P.
 Proof.
-  iIntros (????) "(#Hinv&Hpending&#HC)".
-  iMod (inv_mut_acc with "Hinv") as (Qs_mut) "(Hinv0&Hclo)"; auto.
-  iDestruct (bi_sch_staged_interp_weak with "Hinv0") as "(#Hwand0&#Hwand1&Hpend&#Hinv0)".
-  iDestruct ("Hinv0" $! (E ∖ ↑N1) with "[]") as "Hinv0'".
-  { iPureIntro. set_solver. }
-  iMod (fupd_level_le with "Hinv0'") as "(H&Hclo')"; first by lia.
-  iDestruct "H" as "[HQ|Hfalse]"; last first.
-  {
-    iSpecialize ("Hwand1" with "[$] [$]").
-    iMod (fupd_level_intro_mask' _ ∅) as "_"; first by set_solver+.
-    iMod (fupd_level_le with "Hwand1") as %[]; lia.
-  }
-  iDestruct "HQ" as "[HQ|HQ]".
+  iIntros (?) "(#Hinv&Hpending&#HC)".
+  iMod (ae_inv_mut_acc _ _ _ _ (▷ P) with "Hinv [Hpending]"); last done.
+  iIntros (Qs) "Hinv0".
+  iDestruct (bi_sch_staged_interp_weak with "Hinv0") as "(#Hwand0&H)".
+  iDestruct "H" as "[HQ|HQ]".
   - iMod (fupd_level_intro_mask' _ E1) as "Hclo''"; auto.
     iDestruct ("Hwand0" with "[$] [$]") as "Hwand".
     iMod (fupd_level_le with "Hwand") as "Hwand"; auto.
@@ -567,94 +259,14 @@ Proof.
     iDestruct "HP" as "[HP|>Hfalse]"; last first.
     { iDestruct (pending_done with "[$] Hfalse") as %[]. }
     iMod (pending_upd_done with "[$]") as "#Hdone".
-    iSpecialize ("Hclo'" with "[HQr]").
-    { iLeft. iRight. iFrame "# ∗". }
-    iMod (fupd_level_le with "Hclo'") as "_"; first by lia.
-    iMod ("Hclo" with "[Hpend]").
-    { iApply bi_sch_staged_interp_weak. iFrame "Hwand0 Hwand1 Hpend Hinv0". }
-    iModIntro; eauto.
+    iModIntro. iSplitR "HP"; last done.
+    iApply bi_sch_staged_interp_weak. iFrame "Hwand0". iFrame "# ∗".
   - iDestruct "HQ" as "(HQr&_&[HP|>Hfalse])"; last first.
     { iDestruct (pending_done with "Hpending [$]") as %[]. }
     iMod (pending_upd_done with "[$]") as "#Hdone".
     iFrame.
-    iSpecialize ("Hclo'" with "[HQr]").
-    { iLeft. iRight. iFrame "# ∗". }
-    iMod (fupd_level_le with "Hclo'") as "_"; first by lia.
-    iMod ("Hclo" with "[Hpend]").
-    { iApply bi_sch_staged_interp_weak. iFrame "Hwand0 Hwand1 Hpend Hinv0". }
-    iModIntro; eauto.
-Qed.
-
-Lemma staged_inv_cancel E k N1 N2 E1 γ P Q Qr:
-  N1 ## N2 →
-  ↑N1 ⊆ E →
-  ↑N2 ⊆ E →
-  staged_value (S k) N1 N2 E1 γ Q Qr P -∗
-  staged_pending 1%Qp γ -∗ |(S k)={E,E}=>
-  ▷ Q ∨ (▷ Qr ∗ ▷ P ∗ C).
-Proof.
-  iIntros (???) "Hval Hpend0".
-  iDestruct "Hval" as (??) "(Hqr&Hcancel&#Hinv&Hval)".
-  iMod (inv_mut_full_acc with "Hval") as "(Hinterp&Hclo)"; auto.
-  iInv "Hinv" as "H" "Hclo'".
-  iDestruct "H" as "[HQ|>Hfalse]"; last first.
-  { iDestruct (pending_done with "Hcancel Hfalse") as %[]. }
-  iDestruct (bi_sch_staged_interp with "Hinterp") as "(#Hwand&_&>Hcancel2&_)".
-  iDestruct "HQ" as "[HQ|HQ]".
-  - iDestruct (pending_join with "[$Hcancel $Hcancel2]") as "Hcancel".
-    iMod (pending_upd_done with "Hcancel") as "Hcancel".
-    iMod ("Hclo'" with "[Hcancel]") as "_".
-    { iRight. eauto. }
-    iMod (pending_upd_done with "Hpend0") as "#Hdone0".
-    iMod (pending_alloc) as (γcancel') "Hc".
-    iMod (inv_alloc' _ N2 _
-        (((True ∨ ((True ∨ staged_done γr) ∗ C ∗ (P ∨ staged_done γ))) ∨ staged_done γcancel'))%I
-        with "[]") as "#Hinv0".
-    { repeat iLeft. auto. }
-    iDestruct (pending_split with "Hc") as "(Hc1&Hc2)".
-    iMod ("Hclo" $! [True%I; (True ∨ staged_done γr)%I;
-                     staged_done γcancel'; staged_pending (1/2)%Qp γcancel'] with "[Hc1]").
-    { rewrite bi_sch_staged_interp.
-      iSplitL ""; [| iSplitL ""].
-      - iIntros "!> HQ' >HC".  iModIntro. iModIntro. iFrame "#". eauto.
-      - iModIntro. iIntros ">H1 >H2". iModIntro. iApply (pending_done with "[$] [$]").
-      - iFrame.
-        rewrite /inv_lvl.
-        iModIntro. iIntros (E0 Hsub).
-        iInv "Hinv0" as "H" "Hclo".
-        iModIntro. iFrame.
-    }
-    iModIntro. eauto.
-  - iDestruct "HQ" as "(HQr&>#HC&HP)".
-    iDestruct "HQr" as "[HQr|>Hfalse]"; last first.
-    { iDestruct (pending_done with "Hqr [$]") as %[]. }
-    iDestruct "HP" as "[HP|>Hfalse]"; last first.
-    { iDestruct (pending_done with "Hpend0 [$]") as %[]. }
-    iMod (pending_upd_done with "Hqr") as "Hqr".
-    iMod (pending_upd_done with "Hpend0") as "#Hdone0".
-    iDestruct (pending_join with "[$Hcancel $Hcancel2]") as "Hcancel".
-    iMod (pending_upd_done with "Hcancel") as "Hcancel".
-    iMod ("Hclo'" with "[Hcancel]") as "_".
-    { iRight. eauto. }
-    iMod (pending_alloc) as (γcancel') "Hc".
-    iMod (inv_alloc' _ N2 _
-        (((True ∨ ((True ∨ staged_done γr) ∗ C ∗ (P ∨ staged_done γ))) ∨ staged_done γcancel'))%I
-        with "[]") as "#Hinv0".
-    { repeat iLeft; auto. }
-    iDestruct (pending_split with "Hc") as "(Hc1&Hc2)".
-    iMod ("Hclo" $! [True%I; (True ∨ staged_done γr)%I;
-                     staged_done γcancel'; staged_pending (1/2)%Qp γcancel'] with "[Hc1]").
-    { rewrite bi_sch_staged_interp.
-      iSplitL ""; [| iSplitL ""].
-      - iIntros "!> HQ' >_".  iModIntro. iModIntro. iFrame "#". eauto.
-      - iModIntro. iIntros ">H1 >H2". iModIntro. iApply (pending_done with "[$] [$]").
-      - iFrame.
-        rewrite /inv_lvl.
-        iModIntro. iIntros (E0 Hsub).
-        iInv "Hinv0" as "H" "Hclo".
-        iModIntro. iFrame.
-    }
-    iModIntro. iRight. iFrame "# ∗".
+    iModIntro.
+    iApply bi_sch_staged_interp_weak. iFrame "Hwand0". iFrame "# ∗".
 Qed.
 
 End inv.
